Thread root inode properties through invariant
Lookup requires that the tree's inode number is the root inode in fsxp,
and that the root be a directory. To guarantee that this property is
stable across interference we need it in the invariant. We prove that
every system call preserves this property automatically so the
obligation is removed entirely from system calls.

src/FSProtocol.v
@@ -36,8 +36,13 @@ Section FilesystemProtocol.
       (DirTreeRep.rep (fsxp P) Pred.emp tree ilist frees mscs)
         (list2nmem (ds!!)).
 
+  Definition root_inode_rep tree :=
+    dirtree_inum tree = FSXPRootInum (fsxp P) /\
+    dirtree_isdir tree = true.
+
   Definition fs_invariant l d_i d hm tree (homedirs: thread_homes) : heappred :=
     (fstree P |-> abs tree *
+     [[ root_inode_rep tree ]] *
      fshomedirs P |-> abs homedirs *
      exists c vd mscs,
        ccache P |-> val c *
@@ -54,7 +59,8 @@ Section FilesystemProtocol.
          fsmem P |-> val mscs)%pred h /\
         (cache_rep d c vd \/ cache_rep d_i c vd) /\
         (l = Free -> d_i = d) /\
-        fs_rep vd hm mscs tree.
+        fs_rep vd hm mscs tree /\
+        root_inode_rep tree.
   Proof.
     unfold fs_invariant; intros.
     SepAuto.destruct_lifts.
@@ -68,7 +74,8 @@ Section FilesystemProtocol.
          ccache P |-> val c *
          fsmem P |-> val mscs)%pred h /\
         (cache_rep d c vd) /\
-        fs_rep vd hm mscs tree.
+        fs_rep vd hm mscs tree /\
+        root_inode_rep tree.
   Proof.
     unfold fs_invariant; intros.
     SepAuto.destruct_lifts.
@@ -87,25 +94,93 @@ Section FilesystemProtocol.
          ccache P |-> val c *
          fsmem P |-> val mscs)%pred h /\
         (cache_rep d c vd) /\
-        fs_rep vd hm mscs tree.
+        fs_rep vd hm mscs tree /\
+        root_inode_rep tree.
   Proof.
     intros; subst.
     edestruct fs_invariant_unfold; repeat deex; descend;
       intuition (subst; eauto).
   Qed.
 
-  (* this isn't used yet, so it's statement might not be a useful variant *)
-  Theorem fs_invariant_refold1 : forall tree homedirs l d_i d c vd hm mscs h,
-      (fstree P |-> abs tree * fshomedirs P |-> abs homedirs *
-       ccache P |-> val c *
-       fsmem P |-> val mscs)%pred h ->
-      cache_rep d_i c vd ->
-      fs_rep vd hm mscs tree ->
-      (l = Free -> d_i = d) ->
-      fs_invariant l d_i d hm tree homedirs h.
+  Lemma root_inode_rep_update : forall tree path subtree,
+      root_inode_rep tree ->
+      (path = nil -> root_inode_rep subtree) ->
+      root_inode_rep (update_subtree path subtree tree).
   Proof.
-    unfold fs_invariant; intros.
-    SepAuto.pred_apply; SepAuto.cancel; eauto.
+    unfold root_inode_rep; intros.
+    destruct path; simpl; auto.
+    destruct tree; simpl; intuition; subst.
+  Qed.
+
+  Lemma root_inode_rep_file : forall tree path subtree inum f,
+      root_inode_rep tree ->
+      find_subtree path tree = Some (TreeFile inum f) ->
+      root_inode_rep (update_subtree path subtree tree).
+  Proof.
+    intros.
+    apply root_inode_rep_update; auto.
+    intros; subst; simpl in *.
+    exfalso.
+    inversion H0; subst.
+    unfold root_inode_rep in *.
+    intuition.
+  Qed.
+
+  Lemma root_inode_rep_dir : forall tree path subtree dnum elems,
+      root_inode_rep tree ->
+      find_subtree path tree = Some (TreeDir dnum elems) ->
+      dirtree_inum subtree = dnum ->
+      dirtree_isdir subtree = true ->
+      root_inode_rep (update_subtree path subtree tree).
+  Proof.
+    intros.
+    apply root_inode_rep_update; auto.
+    intros; subst; simpl in *.
+    inversion H0; subst.
+    unfold root_inode_rep in *; intuition.
+  Qed.
+
+  Local Lemma root_inode_rep_refold : forall tree,
+      dirtree_inum tree = FSLayout.FSXPRootInum (fsxp P) ->
+      dirtree_isdir tree = true ->
+      root_inode_rep tree.
+  Proof.
+    unfold root_inode_rep; intuition.
+  Qed.
+
+  Hint Resolve root_inode_rep_refold.
+
+  Ltac simp :=
+    repeat match goal with
+           | _ => solve [ auto ]
+           | _ => progress intros
+           | [ H: Some _ = Some _ |- _ ] =>
+             inversion H; subst; clear H
+           | [ H: TreeDir _ _ = TreeDir _ _ |- _ ] =>
+             inversion H; subst; clear H
+           | _ => progress subst
+           | _ => progress simpl in *
+           end.
+
+  Lemma root_inode_rep_rename:
+    forall (dnum : nat) (srcpath dstpath : list string) (tree : dirtree)
+      (tree_elem : list (string * dirtree)),
+      root_inode_rep tree ->
+      forall (srcnum : nat) (srcents : list (string * dirtree)) (dstnum : nat)
+        (dstents : list (string * dirtree)),
+        find_subtree srcpath (TreeDir dnum tree_elem) = Some (TreeDir srcnum srcents) ->
+        forall (cwd : list string) (tree_ents'' tree_ents' : list (string * dirtree)),
+          find_subtree dstpath (update_subtree srcpath (TreeDir srcnum tree_ents') (TreeDir dnum tree_elem)) =
+          Some (TreeDir dstnum dstents) ->
+          find_subtree cwd tree = Some (TreeDir dnum tree_elem) ->
+          root_inode_rep (update_subtree cwd
+                                         (update_subtree dstpath (TreeDir dstnum tree_ents'')
+                                                         (update_subtree srcpath (TreeDir srcnum tree_ents') (TreeDir dnum tree_elem))) tree).
+  Proof.
+    intros.
+    unfold root_inode_rep in *|-; intuition.
+    eapply root_inode_rep_update; simp.
+    destruct dstpath, srcpath; simp.
   Qed.
 
   Notation "'fs_inv' ( sigma , tree , homedirs )" :=
@@ -211,6 +286,22 @@ Section FilesystemProtocol.
     eapply fs_rely_invariant; eauto.
   Qed.
 
+  Theorem homedir_guarantee_rely : forall tid homedirs tree tree',
+      Relation_Operators.clos_refl_trans
+        _ (fun tree tree' =>
+             exists tid', tid <> tid' /\
+                     homedir_guarantee tid' homedirs tree tree') tree tree' ->
+      homedir_rely tid homedirs tree tree'.
+  Proof.
+    intros.
+    apply Operators_Properties.clos_rt_rt1n in H.
+    induction H.
+    unfold homedir_rely; auto.
+    deex.
+    specialize (H2 tid); intuition.
+    unfold homedir_rely in *; congruence.
+  Qed.
+
   Theorem fs_homedir_rely : forall tid sigma sigma' tree homedirs tree',
       fs_inv(sigma, tree, homedirs) ->
       Rely fs_guarantee tid sigma sigma' ->
@@ -225,7 +316,7 @@ Section FilesystemProtocol.
     - reflexivity.
     - match goal with
       | [ H: homedir_guarantee _ _ _ _ |- _ ] =>
-        specialize (H _ ltac:(eauto))
+        specialize (H _ ltac:(intuition eauto))
       end.
       specialize (IHclos_refl_trans_1n _ ltac:(eauto) _ ltac:(eauto)).
       unfold homedir_rely in *; congruence.
